\documentclass{article}
\usepackage{amsmath}
\usepackage{amssymb}
\usepackage[T1,T2A]{fontenc}
\usepackage[utf8]{inputenc}
\usepackage[bulgarian]{babel}
\usepackage[normalem]{ulem}
\newcommand{\stkout}[1]{\ifmmode\text{\sout{\ensuremath{#1}}}\else\sout{#1}\fi}

\begin{document}
    \pagenumbering{gobble}
    \begin{math}
        \\
        \text{а)} \lim_{n \to \infty} \frac{2n^3 + 3n + 5}{-3n^3 + 4n + 7}\\
        \\
        \lim_{n \to \infty} \frac{2n^3 + 3n + 5}{-3n^3 + 4n + 7}\\
        \\
        \lim_{n \to \infty} \frac{\stkout{n^3}(2 + \frac{3}{n^2} + \frac{5}{n^3})}{\stkout{n^3}(-3 + \frac{4}{n^2} + \frac{7}{n^3})}\\
        \\
        \lim_{n \to \infty} \frac{2 + \frac{3}{n^2} + \frac{5}{n^3}}{-3 + \frac{4}{n^2} + \frac{7}{n^3}}\\
        \\
        \lim_{n \to \infty} \frac{2 + 3\frac{1}{n}\frac{1}{n} + 5\frac{1}{n}\frac{1}{n}\frac{1}{n}}{-3 + 4\frac{1}{n}\frac{1}{n} + 7\frac{1}{n}\frac{1}{n}\frac{1}{n}}\\
        \\
        \frac{1}{n} \to 0 \implies \lim_{n \to \infty} \frac{2 + 3\times0 + 5\times0}{-3 + 4\times0 + 7\times0}\\
        \\
        \implies \lim_{n \to \infty} \frac{2n^3 + 3n + 5}{-3n^3 + 4n + 7} = \frac{-2}{3}\\
        \\
        \\
        \text{б)} \lim_{n \to \infty} \frac{3n^4 + 4^nn^2 + (-3)^n}{2n^3 + 5^n}\\
        \\
        \lim_{n \to \infty} \frac{3n^4 + 4^nn^2 + (-3)^n}{2n^3 + 5^n}\\
        \\
        \lim_{n \to \infty} \frac{3n^4}{2n^3 + 5^n}\\
        \\
        \lim_{n \to \infty} \frac{n^{\stkout{4}}3}{n^{\stkout{3}}(2 + \frac{5^n}{n^3})}\\
        \\
        \lim_{n \to \infty} \frac{3n}{2 + \frac{5^n}{n^3}}\\
        \\
        \ n \to \infty \quad n^3 \prec 5^n \implies \frac{5^n}{n^3} \to \infty \quad n \prec \frac{5^n}{n^3} \implies \lim_{n \to \infty} \frac{3n^4}{2n^3 + 5^n} = 0\\
        \\
        \lim_{n \to \infty} \frac{4^nn^2}{2n^3 + 5^n}\\
        \\
        \lim_{n \to \infty} \frac{n^{\stkout{2}}\frac{4^n}{n^2}}{n^{\stkout{3}}(2 + \frac{5^n}{n^3})}\\
        \\
        \lim_{n \to \infty} \frac{\frac{4^n}{n^2}}{2n + \frac{5^n}{n^2}}\\
        \\
        \ n \to \infty \quad 4^n \prec 5^n\,,\, n^0 \prec 2n \implies \lim_{n \to \infty} \frac{4^nn^2}{2n^3 + 5^n} = 0\\
        \\
        \lim_{n \to \infty} \frac{(-3)^n}{2n^3 + 5^n}\\
        \\
        n \to \infty \quad (-3)^n \to -\infty\,,\, 5^n \to \infty\\
        \\
        (-3)^n \prec 5^n\,,\, n^0 \prec 2n^3 \implies \lim_{n \to \infty} \frac{(-3)^n}{2n^3 + 5^n} = 0\\
        \\
        \lim_{n \to \infty} \frac{3n^4 + 4^nn^2 + (-3)^n}{2n^3 + 5^n} = \lim_{n \to \infty} \frac{3n^4}{2n^3 + 5^n} + \lim_{n \to \infty} \frac{4^nn^2}{2n^3 + 5^n}\\ + \lim_{n \to \infty} \frac{(-3)^n}{2n^3 + 5^n} = 0 + 0 + 0 = 0\\
        \\
        \\
        \text{в)} \lim_{n \to \infty} \frac{n^2 + 3n + 3}{n^2 - 3n -4}^{3n + 3}\\
        \\
        \lim_{n \to \infty} \frac{n^2 + 3n + 3}{n^2 - 3n -4}^{3n + 3}\\
        \\
        \frac{n^2 + 3n + 3}{n^2 - 3n -4} = \frac{\stkout{n^2}(1 + \frac{3}{n} + \frac{3}{n^2})}{\stkout{n^2}(1 - \frac{3}{n} - \frac{4}{n^2}} = \frac{1 + 3\frac{1}{n} + 3\frac{1}{n}\frac{1}{n}}{1 - 3\frac{1}{n}\frac{1}{n} - 4\frac{1}{n}\frac{1}{n}}\\
        \\
        \frac{1}{n} \to 0 \implies \frac{1 + 3\frac{1}{n} + 3\frac{1}{n}\frac{1}{n}}{1 - 3\frac{1}{n}\frac{1}{n} - 4\frac{1}{n}\frac{1}{n}} \to 1
        \\
        \lim_{n \to \infty} \left[1 + \left(\frac{n^2 + 3n + 3}{n^2 - 3n -4} - 1\right)\right]^{3n + 3}\\
        \\
        \lim_{n \to \infty} \left[1 + \left(\frac{n^2 + 3n + 3}{n^2 - 3n -4} - \frac{n^2 - 3n -4}{n^2 - 3n -4}\right)\right]^{3n + 3}\\
        \\
        \lim_{n \to \infty} \left(1 + \frac{6n + 7}{n^2 - 3n -4}\right)^{3n + 3}\\
        \\
        \lim_{n \to \infty} \left[\left(1 + \frac{6n + 7}{n^2 - 3n -4}\right)^{\frac{n^2 - 3n -4}{6n + 7}}\right]^{\frac{6n + 7}{n^2 - 3n -4}3n + 3}\\
        \\
        \lim_{n \to \infty} \left[\left(1 + \frac{6n + 7}{n^2 - 3n -4}\right)^{\frac{n^2 - 3n -4}{6n + 7}}\right]^{\frac{18n^2 + 39n + 21}{n^2 - 3n -4}}\\
        \\
        \left(1 + \frac{6n + 7}{n^2 - 3n -4}\right)^{\frac{n^2 - 3n -4}{6n + 7}} \to e\\
        \\
        \frac{18n^2 + 39n + 21}{n^2 - 3n -4} = \frac{\stkout{n^2}(18 + \frac{39}{n} + \frac{21}{n^2})}{\stkout{n^2}(1 - \frac{3}{n} - \frac{4}{n})} = \frac{18 + 39\frac{1}{n} + 21\frac{1}{n}\frac{1}{n}}{1 - 3\frac{1}{n}\frac{1}{n} - 4\frac{1}{n}\frac{1}{n}}\\
        \\
        \frac{1}{n} \to 0 \implies \frac{18 + 39\frac{1}{n} + 21\frac{1}{n}\frac{1}{n}}{1 - 3\frac{1}{n}\frac{1}{n} - 4\frac{1}{n}\frac{1}{n}} \to 18\\
        \\
        \implies \lim_{n \to \infty} \frac{n^2 + 3n + 3}{n^2 - 3n -4}^{3n + 3} = e^{18}\\
        \\
        \\
        \text{г)} \lim_{n \to \infty} \frac{n^2 + 3n + 3}{n^2 - 3n -4}^{\frac{1}{3n + 3}}\\
        \\
        \lim_{n \to \infty} \frac{n^2 + 3n + 3}{n^2 - 3n -4}^{\frac{1}{3n + 3}}\\
        \\
        \frac{n^2 + 3n + 3}{n^2 - 3n -4} = \frac{\stkout{n^2}(1 + \frac{3}{n} + \frac{3}{n^2})}{\stkout{n^2}(1 - \frac{3}{n} - \frac{4}{n^2}} = \frac{1 + 3\frac{1}{n} + 3\frac{1}{n}\frac{1}{n}}{1 - 3\frac{1}{n}\frac{1}{n} - 4\frac{1}{n}\frac{1}{n}}\\
        \\
        \frac{1}{n} \to 0 \implies \frac{1 + 3\frac{1}{n} + 3\frac{1}{n}\frac{1}{n}}{1 - 3\frac{1}{n}\frac{1}{n} - 4\frac{1}{n}\frac{1}{n}} \to 1
        \\
        \lim_{n \to \infty} \left[1 + \left(\frac{n^2 + 3n + 3}{n^2 - 3n -4} - 1\right)\right]^{\frac{1}{3n + 3}}\\
        \\
        \lim_{n \to \infty} \left[1 + \left(\frac{n^2 + 3n + 3}{n^2 - 3n -4} - \frac{n^2 - 3n -4}{n^2 - 3n -4}\right)\right]^{\frac{1}{3n + 3}}\\
        \\
        \lim_{n \to \infty} \left(1 + \frac{6n + 7}{n^2 - 3n -4}\right)^{\frac{1}{3n + 3}}\\
        \\
        \lim_{n \to \infty} \left[\left(1 + \frac{6n + 7}{n^2 - 3n -4}\right)^{\frac{n^2 - 3n -4}{6n + 7}}\right]^{\frac{6n + 7}{n^2 - 3n -4}{\frac{1}{3n + 3}}}\\
        \\
        \lim_{n \to \infty} \left[\left(1 + \frac{6n + 7}{n^2 - 3n -4}\right)^{\frac{n^2 - 3n -4}{6n + 7}}\right]^{\frac{6n + 7}{3n^3 - 6n^2 - 21n - 12}}\\
        \\
        \left(1 + \frac{6n + 7}{n^2 - 3n -4}\right)^{\frac{n^2 - 3n -4}{6n + 7}} \to e\\
        \\
        \frac{6n + 7}{3n^3 - 6n^2 - 21n - 12} = \frac{\stkout{n}(6 + \frac{7}{n})}{n^{\stkout{3}}(3 - \frac{6}{n} - \frac{21}{n^2} - \frac{12}{n^3})} = \frac{1}{n}\frac{1}{n}\left(\frac{6 + 7\frac{1}{n}}{3 - 6\frac{1}{n} - 21\frac{1}{n}\frac{1}{n} - 12\frac{1}{n}\frac{1}{n}\frac{1}{n}}\right)\\
        \\
        \frac{1}{n} \to 0 \implies \frac{1}{n}\frac{1}{n}\left(\frac{6 + 7\frac{1}{n}}{3 - 6\frac{1}{n} - 21\frac{1}{n}\frac{1}{n} - 12\frac{1}{n}\frac{1}{n}\frac{1}{n}}\right) \to 0\\
        \\
        \implies \lim_{n \to \infty} \frac{n^2 + 3n + 3}{n^2 - 3n -4}^{\frac{1}{3n + 3}} = e^{0} = 1\\
        \\
        \\
        \text{д)} \lim_{n \to \infty} \frac{n}{\sqrt{n^4 + 3n^2 + 4} - \sqrt{n^4 - n^3 + 1}}\\
        \\
        \lim_{n \to \infty} \frac{n}{\sqrt{n^4 + 3n^2 + 4} - \sqrt{n^4 - n^3 + 1}}\\
        \\
        \lim_{n \to \infty} \frac{n}{\sqrt{n^4 + 3n^2 + 4} - \sqrt{n^4 - n^3 + 1}}\frac{\sqrt{n^4 + 3n^2 + 4} + \sqrt{n^4 - n^3 + 1}}{\sqrt{n^4 + 3n^2 + 4} + \sqrt{n^4 - n^3 + 1}}\\
        \\
        \lim_{n \to \infty} \frac{n(\sqrt{n^4 + 3n^2 + 4} + \sqrt{n^4 - n^3 + 1})}{(\sqrt{n^4 + 3n^2 + 4})^2 - (\sqrt{n^4 - n^3 + 1})^2}\\
        \\
        \lim_{n \to \infty} \frac{n\sqrt{n^4}(\sqrt{1 + \frac{3}{n^2} + \frac{4}{n^4}} + \sqrt{1 - \frac{1}{n} + \frac{1}{n^4}})}{(n^4 + 3n^2 + 4) - (n^4 - n^3 + 1)}\\
        \\
        \lim_{n \to \infty} \frac{n^3(\sqrt{1 + \frac{3}{n^2} + \frac{4}{n^4}} + \sqrt{1 - \frac{1}{n} + \frac{1}{n^4}})}{n^3 + 3n^2 + 3}\\
        \\
        \lim_{n \to \infty} \frac{\stkout{n^3}(\sqrt{1 + \frac{3}{n^2} + \frac{4}{n^4}} + \sqrt{1 - \frac{1}{n} + \frac{1}{n^4}})}{\stkout{n^3}(1 + \frac{3}{n} + \frac{3}{n^3})}\\
        \\
        \lim_{n \to \infty} \frac{\sqrt{1 + 3\frac{1}{n}\frac{1}{n} + 4\frac{1}{n}\frac{1}{n}\frac{1}{n}\frac{1}{n}} + \sqrt{1 - \frac{1}{n} + \frac{1}{n}\frac{1}{n}\frac{1}{n}\frac{1}{n}}}{1 + 3\frac{1}{n} + 3\frac{1}{n}\frac{1}{n}\frac{1}{n}}\\
        \\
        \frac{1}{n} \to 0 \implies \lim_{n \to \infty} \frac{\sqrt{1 + 3\times0 + 4\times0} + \sqrt{1 - 0 + 0}}{1 + 3\times0 + 3\times0}\\
        \\
        \implies \lim_{n \to \infty} \frac{n}{\sqrt{n^4 + 3n^2 + 4} - \sqrt{n^4 - n^3 + 1}} = 2\\
        \\
        \\
        \text{е)} \lim_{n \to \infty} \frac{(2n)!!}{(2n)^n}\\
        \\
        \lim_{n \to \infty} \frac{(2n)!!}{(2n)^n}\\
        \\
        \lim_{n \to \infty} \frac{\stkout{2n}(n!)}{\stkout{2n}(2n)^{n - 1}}\\
        \\
        \lim_{n \to \infty} \frac{\displaystyle\prod_{k=1}^{n} k}{\displaystyle\prod_{i=1}^{n - 1} 2n}\\
        \\
        \\
        \displaystyle\prod_{k=1}^{n} k \prec \displaystyle\prod_{i=1}^{n - 1} 2n \implies \lim_{n \to \infty} \frac{(2n)!!}{(2n)^n} = 0
    \end{math}
\end{document}