\documentclass{article}
\usepackage{amsmath}
\usepackage{amssymb}
\usepackage[T1,T2A]{fontenc}
\usepackage[utf8]{inputenc}
\usepackage[bulgarian]{babel}

\begin{document}
    \pagenumbering{gobble}
    \begin{math}
        \\
        1 ^ 3 + 3 ^ 3 + 5 ^ 3 + \dots + (2n - 1) ^ 3 =?\, n ^ 2(2n ^ 2 - 1), n = 1, 2, 3, \dots\\
        \\
        n = 1 \implies 1 ^ 3 =?\, 1 ^ 2(2(1 ^ 2) - 1)\\
        1 ^ 3 = 1\\
        1 ^ 2(2(1 ^ 2) - 1) = 1(2 - 1) = 1\\
        1 = 1\\
        \\
        n = k \implies 1 ^ 3 + 3 ^ 3 + 5 ^ 3 + \dots + (2k - 1) ^ 3 = k ^ 2(2k ^ 2 - 1)\\
        \\
        n = k + 1 \implies 1 ^ 3 + 3 ^ 3 + 5 ^ 3 + \dots + (2(k + 1) - 1) ^ 3 =?\, (k + 1) ^ 2(2(k + 1) ^ 2 - 1)\\
        \\
        1 ^ 3 + 3 ^ 3 + 5 ^ 3 + \dots + (2k - 1) ^ 3 + (2(k + 1) - 1)\\
        = k ^ 2(2k ^ 2 - 1) + (2k + 2 - 1) ^ 3\\
        = 2k^4 - k^2 + (2k + 1) ^ 3\\
        = 2k^4 - k^2 + 8k ^ 3 + 12k ^ 2 + 6k + 1\\
        = 2k^4 + 8k ^ 3 + 11k ^ 2 + 6k + 1\\
        \\
        (k + 1) ^ 2(2(k + 1) ^ 2 - 1)\\
        = (k ^ 2 + 2k + 1)(2(k ^ 2 + 2k + 1) - 1)\\
        = (k ^ 2 + 2k + 1)(2k ^ 2 + 4k + 1)\\
        = 2k ^ 4 + 4k ^ 3 + k ^ 2 + 4k ^ 3 + 8k ^ 2 + 2k + 2k ^ 2 + 4k + 1\\
        2k ^ 4 + 8k ^ 3 + 11k ^ 2 + 6k + 1\\
        \\
        \implies 1 ^ 3 + 3 ^ 3 + 5 ^ 3 + \dots + (2(k + 1) - 1) ^ 3 = (k + 1) ^ 2(2(k + 1) ^ 2 - 1)\\
        \implies 1 ^ 3 + 3 ^ 3 + 5 ^ 3 + \dots + (2n - 1) ^ 3 = n ^ 2(2n ^ 2 - 1), n = 1, 2, 3, \dots
    \end{math}
\end{document}