\documentclass[12pt]{article}
\usepackage{amsmath}
\usepackage{amssymb}
\usepackage{amsthm}
\usepackage{stmaryrd}
\usepackage[T1,T2A]{fontenc}
\usepackage[utf8]{inputenc}
\usepackage[bulgarian]{babel}
\usepackage[normalem]{ulem}
\usepackage[margin=0.5in, top=1cm, left=0.5in]{geometry}
\newcommand{\stkout}[1]{\ifmmode\text{\sout{\ensuremath{#1}}}\else\sout{#1}\fi}
\newcommand{\Z}{\mathbb{Z}}
\newcommand{\N}{\mathbb{N}}
\newcommand{\Cmp}{\mathbb{C}}
\newcommand{\lcm}[2]{\lbrack #1, #2 \rbrack}
\newcommand{\cycleG}[1]{\langle #1 \rangle}

\DeclareMathSizes{12}{14}{12}{8}

\title{Домашна работа 1, №45342, група 3, Информатика}
\author{Иво Стратев}

\begin{document}
    \pagenumbering{gobble}
    \maketitle
    \section*{Задача 1.}
    \(\left\vert\begin{array}{lr}
    	35x + 24 \equiv 0 & \pmod{17} \\
    	23x + 47 \equiv 0 & \pmod{38} \\
    \end{array}\right. \\\\\\
    35x + 24 \equiv 0 \; \pmod{17} \iff 35x + 24 = 17k, \; k \in \Z \\\\
    x = \frac{17k - 24}{35} = m, \; m \in \Z \\\\
    k = \frac{35m + 24}{17} = 2m + 1 + \frac{m + 7}{17} \\\\
    \frac{m + 7}{17} = t, \; t \in \Z \\\\
    m = 17t - 7 \\\\
    x = m = 17t - 7 \implies x \equiv -7 \; \pmod{17} \\\\\\
    23x + 47 \equiv 0 \; \pmod{38} \iff 23x + 47 = 38h, \; h \in \Z \\\\
    x = \frac{38h - 47}{23} = h - 2 + \frac{15h - 1}{23} \\\\
    \frac{15h - 1}{23} = t, \; t \in \Z \\\\
    h = \frac{23t + 1}{15} = t + \frac{8t + 1}{15} \\\\
    \frac{8t + 1}{15} = u, \; u \in \Z \\\\
    t = \frac{15u - 1}{8} = u + \frac{7u - 1}{8} \\\\
    \frac{7u - 1}{8} = r, \; r \in \Z \\\\
    u = \frac{8r + 1}{7} = r + \frac{r + 1}{7} \\\\
    \frac{r + 1}{7} = z, \; z \in \Z \\\\
    r = 7z - 1 \\\\
    u = 7z - 1 + z = 8z - 1 \\\\
    t = 8z - 1 + 7z - 1 = 15z - 2 \\\\
    h = 15z - 2 + 8z -1 = 23z - 3 \\\\
    x = 23z - 3 - 2 + 15z -2 = 38z - 7 \implies x \equiv -7 \; \pmod{38} \)
    \section*{Тв. 1.}
    \(a, b \in \Z, \; n, m \in \N \; a \equiv b \; \pmod{n}, a \equiv b \; \pmod{m} \implies a \equiv b \; \pmod{[m,n]}\)
    \subsection*{Док-во.}
    \(m | [m, n], n | [m, n], \; \forall k \in \Z; \; m | k, \; n | k \implies [m, n] | k \\\\
    a \equiv b \; \pmod{n} \implies n | (a - b) \\\\
    a \equiv b \; \pmod{m} \implies m | (a - b) \\\\
    \implies [m, n] | (a - b) \implies  a \equiv b \; \pmod{[m,n]} \qed\)
    \\\\ \(\left\vert\begin{array}{lr}
    	x \equiv -7 & \pmod{17} \\
    	x \equiv -7 & \pmod{38} \\
    \end{array}\right. \implies x \equiv -7 \; \pmod{[17,38]} \\\\\\
    38 = 2.17 + 4 \\\\
    17 = 4.4 + 1 \\\\
    4 = 1.4 + 0 \implies (38, 17) = 1 \implies \\\\
    \lcm{38}{17} = \frac{38.17}{1} = 646 \implies x \equiv -7 \; \pmod{646} \)
    \\\\ Отговор: \(x \equiv -7 \; \pmod{646} \)
    \section*{Задача 2.}
    \(437^{101} + 403^{201} \equiv \; ? \; \pmod{1000} \\\\
    1000 = 125.8 = 2^3.5^3 \\\\
    437 = 3.125 + 62 \\\\
    125 = 2.62 + 1 \\\\
    62 = 1.62 + 0 \implies (437, 125) = (437, 5^3) = 1 \\\\
    437 = 54.8 + 5 \\\\
    8 = 1.5 + 3 \\\\
    5 = 1.3 + 2 \\\\
    3 = 1.2 + 1 \\\\
    2 = 1.1 + 0 \implies (437, 8) = (437, 2^3) = 1 \)
    \section*{Тв. 2.}
    \(n, k \in \N \; \varphi(n^k) = n^k - n^{k - 1} \)
    \subsection*{Док-во.}
    \(D = [0, \dots, n^k - 1] \subset \N \implies |D| = n^k \\\\
    D = \{mn + r \; | \; m, r \in \N \cup \{0\}, \; 0 \leq r < n, \; 0 \leq mn + r < n^k\} \\\\
    M = \{mn \; | \; m \in \N \cup \{0\}, \; 0 \leq mn < n^k\} \implies |M| = \frac{|D|}{n} = \frac{n^k}{n} = n^{k - 1} \\\\
    P = \{mn + r \; | \; m, r \in \N \cup \{0\}, \; 1 \leq r < n, \; 0 \leq mn + r < n^k\} \implies \\\\
    P = D \backslash M \implies |P| = |D \backslash M| \implies = |D| - |M| = n^k - n^{k - 1} \\\\
    \varphi(n^k) = |P| = n^k - n^{k - 1} \qed \\\\
    \implies \text{ От Th на Ойлер-Ферма } \\\\
    437^{\varphi(2^3)} \equiv 1 \; \pmod{8} \implies 437^{4} \equiv 1 \; \pmod{8} \\\\
    437^{\varphi(5^3)} \equiv 1 \; \pmod{125} \implies 437^{100} \equiv 1 \; \pmod{125} \)
    \section*{Тв. 3.}
    \(a, b \in \Z, \; m, n \in \N \; a \equiv b \; \pmod{m} \implies a^n \equiv b^n \; \pmod{m}\)
    \subsection*{Док-во.}
    \(a \equiv b \; \pmod{m} \implies m | (a - b) \iff
    \left\vert\begin{array}{l}
    	a = a_1.m + r \\
    	b = b_1.m + r
    \end{array}\right. \; a_1, b_1, r \in \Z ; \; 0 \leq r < |m| \\\\
    \implies a - b = a_1.m + r - (b_1.m + r) = (a_1 - b_1)m + (r - r) = (a_1 - b_1)m \\\\
    a^n = (r + a_1.m)^n = \displaystyle\sum_{k = 0}^n \binom{n}{k} r^{n - k}(a_1.m)^k \\\\
    b^n = (r + b_1.m)^n = \displaystyle\sum_{k = 0}^n \binom{n}{k} r^{n - k}(b_1.m)^k \\\\
    a^n - b^n = \displaystyle\sum_{k = 0}^n \binom{n}{k} r^{n - k}.m^k.(a_1^k - b_1^k) = \\\\
    = \binom{n}{0} r^{n}.m^0.(a_1^0 - b_1^0) + \displaystyle\sum_{k = 1}^n \binom{n}{k} r^{n - k}.m^k.(a_1^k - b_1^k) = \\\\
    = r^k - r^k +  \displaystyle\sum_{k = 1}^n \binom{n}{k} r^{n - k}.m^k.(a_1^k - b_1^k) = \\\\
    = \displaystyle\sum_{k = 1}^n \binom{n}{k} r^{n - k}.m^k.(a_1^k - b_1^k) \implies \\\\\\
    m | (a^n - b^n) \implies a^n \equiv b^n \; \pmod{m} \qed \\\\
    \implies (437^4)^{25} \equiv 1^{25} \; \pmod{8} \implies 437^{100} \equiv 1 \; \pmod{8} \\\\
    \implies 437^{100} \equiv 1 \; \pmod{[8, 125]} \implies 437^{100} \equiv 1 \; \pmod{1000} \)
    \section*{Тв. 4.}
    \(a, b, z \in \Z, \; m \in \N; \; a \equiv b \; \pmod{m} \implies za \equiv zb \; \pmod{m}\)
    \subsection*{Док-во.}
    \(a \equiv b \; \pmod{m} \implies m | (a - b) \implies \\\\
    m | z(a - b) \implies m | (za - zb) \implies za \equiv zb \; \pmod{m} \qed \\\\
    \implies 437.437^{100} \equiv 437.1 \; \pmod{1000} \implies 437^{101} \equiv 437 \; \pmod{1000} \\\\
    403 = 3.125 + 28 \\\\
    125 = 4.28 + 13 \\\\
    28 = 2.13 + 2 \\\\
    13 = 6.2 + 1 \\\\
    2 = 1.2 + 0 \implies (403, 125) = (403, 5^3) = 1 \\\\
    403 = 50.8 + 3 \\\\
    8 = 2.3 + 2 \\\\
    3 = 1.2 + 1 \\\\
    2 = 1.1 + 0 \implies (437, 8) = (437, 2^3) = 1 \\\\
    403^{\varphi(2^3)} \equiv 1 \; \pmod{8} \implies 403^{4} \equiv 1 \; \pmod{8} \\\\
    403^{\varphi(5^3)} \equiv 1 \; \pmod{125} \implies 403^{100} \equiv 1 \; \pmod{125} \\\\
    (403^4)^{50} \equiv 1^{50} \; \pmod{8} \implies 403^{200} \equiv 1 \; \pmod{8} \\\\
    (403^{100})^{2} \equiv 1^{2} \; \pmod{125} \implies 403^{200} \equiv 1 \; \pmod{125} \\\\
    403^{200} \equiv 1 \; \pmod{[8, 125]} \implies 437^{200} \equiv 1 \; \pmod{1000} \\\\
    403.403^{200} \equiv 403.1 \; \pmod{1000} \implies 403^{201} \equiv 403 \; \pmod{1000} \)
    \section*{Тв. 5.}
    \(a, b, c, d \in \Z, \; m \in \N \; \left\vert\begin{array}{l}
    	a \equiv b \; \pmod{m} \\
    	c \equiv d \; \pmod{m}
    \end{array}\right. \implies (a + c) \equiv (b + d) \; \pmod{m} \)
    \subsection*{Док-во.}
    \(a \equiv b \; \pmod{m} \implies m | (a - b) \implies a - b = km , \; k \in \Z \\\\
     c \equiv d \; \pmod{m} \implies m | (c - d) \implies c - d = nm , \; n \in \Z \\\\
    (a + c) - (b + d) = (a - b) + (c - d) = km - nm = (k - n)m \implies \\\\
    m | \lbrack (a + c) - (b + d) \rbrack \implies (a + c) \equiv (b + d) \; \pmod{m} \qed \\\\
    \implies  437^{101} + 403^{201} \equiv 437 + 403 \; \pmod{1000} \implies \\\\
    437^{101} + 403^{201} \equiv 840 \; \pmod{1000} \)
    \\\\ Отговор: \(840 \)
    \section*{Задача 3.}
    \((J, \circ_J), \; (C, \circ_C) \\\\
    J \times C = \{(j, c) \; | \; j \in J, \; c \in C\} \\\\
    (j_1, c_1) \circ (j_2, c_2) = (j_1 \circ_J j_2, c_1 \circ_C c_2) \\\\\\
    \forall (j_1, j_2), (c_1, c_2) \in J \times C \; (j_1, c_1) \circ (j_2, c_2) = (j_1 \circ_J j_2, c_1 \circ_C c_2) \\\\
    j_1 \circ_J j_2 \in J \; ( \quad j_1, j_2 \in J, \; (J, \circ_J) \quad ) \\\\
    c_1 \circ_C c_2 \in C \; ( \quad c_1, c_2 \in C, \; (C, \circ_C) \quad ) \\\\
    \implies \forall (j_1, c_1), (j_2, c_2) \in J \times C \implies (j_1, c_1) \circ (j_2, c_2) \in J \times C \)
    \subsection*{а)}
    \(\forall (j_1, c_1), (j_2, c_2), (j_3, c_3) \in J \times C \\
    ((j_1, c_1) \circ (j_2, c_2)) \circ (j_3, c_3) = (j_1 \circ_J j_2, c_1 \circ_C c_2) \circ (j_3, c_3) = \\\\
    = ((j_1 \circ_J j_2) \circ_J j_3, (c_1 \circ_C c_2) \circ_C c_3) = (j_1 \circ_J (j_2 \circ_J j_3), c_1 \circ_C (c_2 \circ_C c_3)) = \\\\
    = (j_1, c_1) \circ (j_2 \circ_J j_3, c_2 \circ_C c_3) = (j_1, c_1) \circ ((j_2, c_2) \circ (j_3, c_3)) \\\\\\
    \forall (j, c) \in J \times C \; (e_G, e_C) \circ (j, c) = (e_J \circ_J j, e_C \circ_C c) = (j, c) = \\\\
    = (j \circ_J e_J, c \circ_C e_C) = (e_J, e_C) \circ (j, c) \implies e = (e_G, e_C) \\\\\\
    \forall (j, c) \; (j, c) \circ (j^{-1}, c^{-1}) = (j \circ_J j^{-1}, c \circ_C c^{-1}) = (e_J, e_C) = \\\\
    = (j^{-1} \circ_J j, c^{-1} \circ_C c) = (j^{-1}, c^{-1}) \circ (j, c) \implies \\\\
    \forall (j, c) \in J \times C \; (j, c)^{-1} = (j^{-1}, c^{-1}) \\\\\\
    \implies (J \times C, \circ) \\\\\\
    |J| < \infty, \; |C| < \infty \implies |J \times C| = |J||C| \)
    \subsection*{б)}
    \subsubsection*{Тв. 6.}
    \(|J| < \infty, \; |C| < \infty, \; J, C - \text{ циклични } \implies J \times C \text{ е циклична } \iff (|J|, |C|) = 1 \)
    \subsubsection*{Док-во.}
    \(|J| < \infty, \; |J| = n \in \N, \; J - \text{ циклична } \implies \\\\
    \exists j \in J; \; |j| = n, \; J = \cycleG{j} = \{j^k \; | \; k \in \Z\} \\\\
    |C| < \infty, \; |C| = m \in \N, \; C - \text{ циклична } \implies \\\\
    \exists c \in C; \; |c| = m, \; C = \cycleG{c} = \{c^k \; | \; k \in \Z\} \\\\\\
    a, b \in \Z \; (j^a, c^b) \in J \times C, k \in \N \quad (j^a, c^b)^k = \underbrace{(j^a, c^b) \circ (j^a, c^b) \circ \dots \circ (j^a, c^b)}_k = \\\\
    = (\underbrace{j^a \circ_J j^a \circ_J \dots \circ_J j^a}_k, \underbrace{c^b \circ_C c^b \circ_C \dots \circ_C c^b}_k) = ((j^a)^k, (c^b)^k) = (j^{ak}, c^{bk}) \\\\
    (j^a, c^b)^{-k} = \underbrace{(j^a, c^b)^{-1} \circ (j^a, c^b)^{-1} \circ \dots \circ (j^a, c^b)^{-1}}_k = \\\\
    = \underbrace{(j^{-a}, c^{-b}) \circ (j^{-a}, c^{-b}) \circ \dots \circ (j^{-a}, c^{-b})}_k = \\\\
    = (\underbrace{j^{-a} \circ_J j^{-a} \circ_J \dots \circ_J j^{-a}}_k, \underbrace{c^{-b} \circ_C c^{-b} \circ_C \dots \circ_C c^{-b}}_k) = \\\\
    = ((j^{-a})^k, (c^{-b})^k) = (j^{-ak}, c^{-bk}) \\\\
    \implies \forall r,t \in Z \; ((j^a, c^b)^r)^t = ((j^{ar}), (c^{ar}))^t = ((j^{ar})^t, (c^{ar})^t) = (j^{art}, c^{brt}) = \\\\
    = ((j^{at})^r, (c^{bt})^r) = ((j^{at}), (c^{bt}))^r = ((j^a, c^b)^t)^r = ((j^{rt})^a, (c^{rt})^b) \\\\
    \implies \forall r,t \in Z \; (j^a, c^b)^r \circ (j^a, c^b)^t = (j^a, c^b)^{r + t} \)
    \subsubsection*{(\(\Rightarrow\))}
    \(J \times C \; \text{ е циклична } \implies \exists y, w \in \Z; \; (j^y, c^w) \in J \times C ; \\\\
    |(j^y, c^w)| = |J \times C| = |J||C|, \; J \times C = \cycleG{(j^y, c^w)} \\\\\\
    d = (n, m) \implies \left\vert\begin{array}{l}
    	d | n \implies 1 \leq d \leq n \\
    	d | m \implies 1 \leq d \leq m
    \end{array}\right. \implies \\\\
    1 \leq d \leq min\{m, n\} \implies \left\vert\begin{array}{l}
    	n = n_1d, \; n_1 \in \N \\
    	m = m_1d, \; n_2 \in \N
    \end{array}\right. \\\\\\
    \text{Доп. } \;  1 < d \leq min\{m, n\} \implies \\\\
    \lcm{m}{n} = \frac{mn}{d} = \frac{m_1dn_1d}{d} = m_1dn_1 \implies \lcm{m}{n} < (m , n) \\\\
    u, v \in \Z, \; (j^u, c^v)^{\lcm{m}{n}} = ((j^u)^{\lcm{m}{n}}, (c^v)^{\lcm{m}{n}}) = (j^{u\lcm{m}{n}}, c^{v\lcm{m}{n}}) = (j^{um_1dn_1}, c^{vm_1dn_1}) \\\\
     = (j^{num_1}, c^{mvn_1}) = ((j^n)^{um_1}, (c^m)^{vn_1}) = (e_J^{um_1}, e_C^{vn_1}) = (e_J, e_C) = e \implies \\\\
    \forall s, z \in \Z \; |(j^s, c^z)| \leq \lcm{m}{n} < (m, n) \implies \lightning \implies \\\\
    d = (m, n) = (|J|, |C|) = 1
    \)
    \subsubsection*{(\(\Leftarrow\))}
    \((m, n) = 1 \implies \lcm{m}{n} = \frac{mn}{(m, n)} = \frac{mn}{1} = mn \\
    (j, c)^n = (j^n, c^n) = (e_J, c^n), \; (m,n) = 1 \implies n = q_1m + 1, \; q_1 \in \Z \implies \\\\
    c^n = c^{q_1m + 1} = c^{q_1m}c = (c^n){q_1}c = e_C^{q_1}c = e_Cc = c \implies \\\\
    (e_J, c^n) = (e_J, c) , \; (e_J, c)^m = (e_J^m, c^m) = (e_J, e_C) = e \\\\
    (m, n) = 1 \implies mn = min\{q \in \N \; | \; (j, c)^q = e \} \implies \\\\
    |(j, c)| = |J \times C| \\\\
    h, l \in \N; 0 \leq h < l < mn \)
    \\\\\\ Доп. \((j, c)^h = (j, c)^l \; | \; (j, c)^{-h} \implies e = (j, c)^{l - h} \implies \\\\
    0 < l - h < mn \implies \lightning \implies (j, c)^h \neq (j, c)^l \\\\
    x \in \Z \; x = q(mn) + x_0, \; q, x_0 \in \Z, \ ; 0 \leq x_0 < mn \implies \\\\
    (j, c)^x = (j, c)^{q(mn) + x_0} = (j, c)^{q(mn)}(j, c)^{x_0} = \\\\
    = ((j, c)^{mn})^q(j, c)^{x_0} = e^q(j, c)^{x_0} = (j, c)^{x_0} = (j^{x_0}, c^{x_0}) \\\\
    \left\vert\begin{array}{l}
    	 x_0 = q_jn + x_j, \; q_j, x_j \in \Z; \; 0 \leq x_j < n \\
    	 x_0 = q_cm + x_c, \; q_c, x_c \in \Z; \; 0 \leq x_c < m \\
    \end{array}\right. \implies \\\\\\
    (j^{x_0}, c^{x_0}) = (j^{q_jn + x_j}, c^{q_cm + x_c}) = (j^{q_jn}j^{x_j}, c^{q_cm}j^{x_c}) = \\\\
    = ((j^n)^{q_j}j^{x_j}, (j^m)^{q_c}c^{x_c}) = (e_J^{q_j}j^{x_j}, e_C^{q_c}c^{x_c}) = (e_Jj^{x_j}, e_Cc^{x_c}) = \\\\
    = (j^{x_j}, c^{x_c}) \in J \times C \implies \left\vert\begin{array}{lr}
    	x \equiv x_j & \pmod{n} \\
    	x \equiv x_c & \pmod{m} \\
    \end{array}\right.\\\\
    \implies J \times C = \cycleG{(j, c)} = \{(j, c)^{k_g} \; | \; k_g \in \Z\} \\\\
    \implies (J, \circ_J), (C, \circ_C); \; J = \cycleG{j}, C = \cycleG{c} \implies \\\\
    (J \times C, \circ) = \cycleG{(j, c)} \iff (|J|, |C|) = 1 \qed\)
    \subsection*{Тв. 7.}
    \(\Cmp_m \times \Cmp_n \cong \Cmp_{mn} \iff (m, n) = 1 \)
    \subsection*{Док-во.} 
    \(\Cmp_m = \cycleG{w_1} = \{1, w_1, w_1^2, \dots, w_1^{m - 1}\}, \; |\Cmp_m| = m \\\\
    \Cmp_n = \cycleG{w_1} = \{1, w_1, w_1^2, \dots, w_1^{n - 1}\}, \; |\Cmp_n| = n \\\\
    (m, n ) = 1 \iff \Cmp_m \times \Cmp_n = \cycleG{w_1, w_1} = \\\\
    = \{(1, 1), (w_1, w_1), (w_1, w_1)^2, \dots, (w_1, w_1)^{mn - 1}\}, \; |\Cmp_m \times \Cmp_n| = mn \\\\
    \Cmp_{mn} = \cycleG{w_1} = \{1, w_1, w_1^2, \dots, w_1^{mn - 1}\}, \; |\Cmp_{mn}| = mn \\\\
    \begin{array}{cccc}
    \varphi : & \Cmp_{mn} & \to & \Cmp_m \times \Cmp_n \\
     ~ &  w_1^k & \mapsto & (w_1, w_1)^k
    \end{array} \quad \quad
    \begin{array}{cccc}
    \varphi^* : & \Cmp_m \times \Cmp_n & \to & \Cmp_{mn} \\
     ~ & (w_1, w_1)^k & \mapsto & w_1^k
    \end{array} \\\\\\
    \varphi(w_1^k) = (w_1, w_1)^k, \; k = 0, 1, \dots, mn - 1 \\\\
    \varphi^*((w_1, w_1)^k) = w_1^k, \; k = 0, 1, \dots, mn - 1 \\\\
    (\varphi \circ \varphi^*)((w_1, w_1)^k) = \varphi(\varphi^*((w_1, w_1)^k) = \varphi(w_1^k) = (w_1, w_1)^k \implies \varphi \circ \varphi^* = id \\\\
    (\varphi^* \circ \varphi)(w_1^k) = \varphi^*(\varphi(w_1^k)) = \varphi^*((w_1, w_1)^k) = w_1^k \implies \varphi^* \circ \varphi = id \\\\
    \implies \varphi^* = \varphi^{-1} \implies \varphi \text{ е биекция } \\\\
    i, j, r \in \N; \; 0 \leq i, j, r < mn, \; i + j \equiv r \; \pmod{mn} \\\\
    \varphi(w_1^i w_1^j) = \varphi(w_1^{i + j}) = \varphi(w_1^r) = (w_1, w_1)^{r} = \\\\
    = (w_1, w_1)^{i + j} = (w_1, w_1)^i(w_1, w_1)^j = \varphi(w_1^i)\varphi(w_1^j) \\\\
    \implies \Cmp_m \times \Cmp_n \cong \Cmp_{mn} \iff (m, n) = 1 \qed \)
    \subsection*{в)}
    \(35 = 3.9 + 8 \\\\
    9 = 1.8 + 1 \\\
    8 = 8.1 + 0 \implies (35, 9) = 1, \; 35.9 = 315 \implies \\\\
    \Cmp_{35} \times \Cmp_9 \cong \Cmp_{315} \)
    \subsection*{г)}
    \(63 = 12.5 + 3 \\\\
    5 = 1.3 + 2 \\\\
    3 = 1.2 + 1 \\\\
    2 = 2.1 = 0 \implies (5, 63) = 1, \; 5.63 = 315 \implies \\\\
    \Cmp_5 \times \Cmp_{63} \cong \Cmp_{315} \implies \exists \tau; \\\\
    \begin{array}{cccc}
    \tau : & \Cmp_{315} & \to & \Cmp_5 \times \Cmp_{63} \\
     ~ &  w_1^k & \mapsto & (w_1, w_1)^k
    \end{array} \quad \quad
    \begin{array}{cccc}
    \tau^{-1} : & \Cmp_5 \times \Cmp_{63} & \to & \Cmp_{315} \\
     ~ & (w_1, w_1)^k & \mapsto & w_1^k
    \end{array} \\\\\\
    47 = 6.7 + 3 \\\\
    7 = 2.3 + 1 \\\\
    3 = 3.1 + 0 \implies (7, 45) = 1, \; 7.45 = 315 \implies \\\\
    \Cmp_7 \times \Cmp_{45} \cong \Cmp_{315} \implies \exists \psi \\\\
    \begin{array}{cccc}
    \psi : & \Cmp_{315} & \to & \Cmp_7 \times \Cmp_{45} \\
     ~ &  w_1^k & \mapsto & (w_1, w_1)^k
    \end{array} \quad \quad
    \begin{array}{cccc}
    \psi^{-1} : & \Cmp_7 \times \Cmp_{45} & \to & \Cmp_{315} \\
     ~ & (w_1, w_1)^k & \mapsto & w_1^k
    \end{array} \implies \\\\\\
    \rho = \psi \circ \tau^{-1} : \Cmp_5 \times \Cmp_{63} \to \Cmp_7 \times \Cmp_{45} \\\\
    \rho((w_1, w_1)_{5 \times 63}^k) = (\psi \circ \tau^{-1})((w_1, w_1)_{5 \times 63}^k) = \psi(\tau^{-1}((w_1, w_1)_{5 \times 63}^k)) = \\\\
    = \psi(w_1^k) = (w_1, w_1)_{7 \times 45}^k \in \Cmp_7 \times \Cmp_{45}, \; k = 0, 1, \dots, mn - 1 \\\\\\
    \rho^{-1} = \tau \circ \psi^{-1} : \Cmp_7 \times \Cmp_{45} \to \Cmp_5 \times \Cmp_{63} \\\\
    \rho((w_1, w_1)_{7 \times 45}^k) = (\psi \circ \tau^{-1})((w_1, w_1)_{7 \times 45}^k) = \psi(\tau^{-1}((w_1, w_1)_{7 \times 45}^k)) = \\\\
    = \psi(w_1^k) = (w_1, w_1)_{5 \times 63}^k \in \Cmp_5 \times \Cmp_{63}, \; k = 0, 1, \dots, mn - 1 \\\\\\
    \rho \circ \rho^{-1} = (\tau \circ \psi^{-1}) \circ (\psi \circ \tau^{-1}) = \tau \circ ((\psi^{-1} \circ \psi) \circ \tau^{-1}) = \\\\
    = \tau \circ (id \circ \tau^{-1}) = \tau \circ \tau^{-1} = id \\\\
    \rho^{-1} \circ \rho = (\psi \circ \tau^{-1}) \circ (\tau \circ \psi^{-1}) = \psi \circ ((\tau^{-1} \circ \tau) \circ \psi^{-1}) = \\\\
    = \psi \circ (id \circ \psi^{-1}) = \psi \circ \psi^{-1} = id \implies \rho \text{ е биекция } \\\\
    i, j, r \in \N; \; 0 \leq i, j, r < mn, \; i + j \equiv r \; \pmod{mn} \\\\
    \rho((w_1, w_1)_{5 \times 63}^i (w_1, w_1)_{5 \times 63}^j) = \rho((w_1, w_1)_{5 \times 63}^{i + j}) = \rho((w_1, w_1)_{5 \times 63}^r) = (w_1, w_1)_{7 \times 45}^{r} = \\\\
    = (w_1, w_1)_{7 \times 45}^{i + j} = (w_1, w_1)_{7 \times 45}^i(w_1, w_1)_{7 \times 45}^j = \rho((w_1, w_1)_{5 \times 63}^i)\rho((w_1, w_1)_{5 \times 63}^j) \\\\
    \implies \Cmp_5 \times \Cmp_{63} \cong \Cmp_7 \times \Cmp_{45} \)
    \subsection*{д)}
    \(JC = \{jc \; | \; j \in J, \; c \in C\}, \; J \triangleleft JC, \; C \triangleleft JC, \; J \cap C = \{1\} \)
    \subsection*{Тв. 8.}
    \(H, G - \text{ групи } H \triangleleft G \implies \forall g \in G, \; \forall h \in H \; ghg^{-1} \in H \)
    \subsection*{Док-во.}
    \(H \triangleleft G \implies \forall g \in G \; gH = Hg \implies \\\\
    h \in H \implies gh \in gH = Hg \implies \exists h^* \in H; \; gh = h^*g \; | \; g^{-1} \implies \\\\
    ghg^{-1} = h^* \in H \implies \forall g \in G, \; \forall h \in H \; ghg^{-1} \in H \qed \\\\\\ \)
    \(j \in J, c \in C, \; J \triangleleft JC, \; C \triangleleft JC \implies JC \ni j, c, j^{-1}, c^{-1} \implies \\\\
    jcj^{-1} \in C, \; cj^{-1}c^{-1} \in J \implies jcj^{-1}c^{-1} \in J \cap C = \{1\} \implies \\\\
    jcj^{-1}c^{-1} = jj^{-1}cc^{-1} = 1.1 = 1 \implies jc = cj \implies \\\\
    \forall y \in J, x \in C \; yx = xy \\\\
    \begin{array}{cccc}
    \sigma : & J \times C  & \to & JC \\
     ~ &  (j, c) & \mapsto & jc
    \end{array} \quad \quad \begin{array}{cccc}
    \sigma^{-1} : & JC & \to & J \times C \\
     ~ &  jc & \mapsto & (j,c)
    \end{array} \\\\\\
    (j_1, c_1), (j_2, c_2) \in J \times C \implies \\\\
    \sigma((j_1, c_1) \circ (j_2, c_2)) = \sigma((j_1j_2, c_1c_2)) = j_1j_2c_1c_2 = \\\\
    = j_1(j_2c_1)c_2 = j_1(c_1j_2)c_2 = (j_1c_1)(j_2c_2) = \sigma((j_1, c_1))\sigma((j_2, c_2)) \\\\
    \sigma^{-1}(jc) = \{(u, v) \in J \times C \; | \; \sigma((u, v)) = jc\} \\\\
    \sigma((u, v)) = jc \iff uv = jc \; | \;  u^{-1} \implies \\\\
    v = u^{-1}jc \; | \; c^{-1} \implies uv = jc \iff vc^{-1} = u^{-1}j = z \\\\
    u, j \in J, \; v, c \in C \implies z \in J \cap C = \{1\} \implies
    \begin{cases}
    	vc^{-1} = 1  \; | \; c \implies v = c \\
    	u^{-1}j = 1  \; | \; u \implies j = u \\
    \end{cases} \implies \\\\
    |\sigma^{-1}(jc)| = |J \cap C| = 1 \implies \sigma \; \text{ е инекция и сюрекция } \implies \sigma \text{ е биекция} \\\\
    \implies JC \cong J \times C\)
    \section*{Задача 4.}
    \((G, .), |G| = n \in \N, p \text{ - просто} \in N, \; p | n \\\\
    M = \{(g_0, g_1, \dots, g_{p - 1}) \in G^p \; | \; g_0.g_1.\dots.g_{p - 1} = e_G \}\)
    \subsection*{а)}
    \(k \in [0, p - 1] \subset N, \; g_0, g_1, \dots g_{k - 1}, g_{k + 1}, \dots, g_{p - 1} \in G \\\\
    g_k = (g_0.g_1.\dots.g_{k - 1})^{-1} (g_{k + 1}.\dots.g_{p - 1})^{-1} = (g_{k - 1}^{-1}.\dots.g_1^{-1}.g_0^{-1})(g_{p - 1}^{-1}.\dots.g_{k + 1}^{-1}) \\\\
    g_0.g_1. \dots.g_{k - 1}.g_k.g_{k + 1}.\dots.g_{p - 1} = \\\\
    = g_0.g_1.\dots.g_{k - 1}g_{k - 1}^{-1}.\dots.g_1^{-1}.g_0^{-1}g_{p - 1}^{-1}.\dots.g_{k + 1}^{-1}.g_{k + 1}.\dots.g_{p - 1} = \\\\
    = \displaystyle\prod_{i = 0}^{k - 1} g_i \displaystyle\prod_{j = k - 1}^{0} g_j^{-1} \displaystyle\prod_{l = p - 1}^{k + 1} g_l^{-1} \displaystyle\prod_{h = k + 1}^{p - 1} g_h =
    \displaystyle\prod_{t = 0}^{p - 1} g_t = e_G \implies \\\\
    \forall k \in [0, p - 1] \subset N, \; \forall g_0, g_1, \dots g_{k - 1}, g_{k + 1}, \dots, g_{p - 1} \in G \implies \\\\
    g_k = \displaystyle\prod_{j = k - 1}^{0} g_j^{-1} \displaystyle\prod_{l = p - 1}^{k + 1} g_l^{-1} \implies \displaystyle\prod_{i = 0}^{p - 1} g_i = e_G \implies \\\\
    (g_0, g_1, \dots, g_{p - 1}) \in M \implies |M| = |G|^{p - 1} = n^{p - 1} \)
    \subsection*{б)}
    \(\begin{array}{cccc}
    \sigma : & M  & \to & G^p \\
     ~ &  (g_0, g_1, \dots, g_{p - 1}) & \mapsto & (g_{p - 1}, g_0, g_1, \dots, g_{p - 2})
    \end{array} \\\\\\
    g \in M \implies g = (g_0, g_1, \dots, g_{p - 1}), \; g_i \in G, \; i = 0, \dots, p - 1 \\\\
    g \in M \implies g_0.g_1.\dots.g_{p - 1} = e_G \; | \; g_{p - 1}^{-1} \implies \\\\
    g_0.g_1.\dots.g_{p - 2} = g_{p - 1}^{-1} \; | \; g_{p - 1} \implies g_{p - 1}.g_0.g_1.\dots.g_{p - 2} = e_G \implies \\\\
    (g_{p - 1}, g_0, g_1, \dots, g_{p - 2}) \in M \\\\
    \sigma(g) = \sigma((g_0, g_1, \dots, g_{p - 1})) = (g_{p - 1}, g_0, g_1, \dots, g_{p - 2}) \implies \sigma : M \to M \\\\
    \begin{array}{cccc}
    \upsilon : & M  & \to & G^p \\
     ~ &  (g_0, g_1, \dots, g_{p - 1}) & \mapsto & (g_1, g_2, \dots, g_{p - 1}, g_0)
    \end{array} \\\\\\
    g_0.g_1.\dots.g_{p - 1} = e_G \; | \; g_0^{-1} \implies \\\\
    g_1.\dots.g_{p - 1} = g_0^{-1} \; | \; g_0 \implies g_1.g_2.\dots.g_{p - 1}.g_0 = e_G \implies \\\\
    (g_1, g_2, \dots, g_{p - 1}, g_0) \in M \\\\
    \upsilon(g) = \upsilon((g_0, g_1, \dots, g_{p - 1})) = (g_1, g_2, \dots, g_{p - 1}, g_0) \implies \upsilon : M \to M \\\\
    (\sigma \circ \upsilon)(g) = \sigma(\upsilon(g)) = \sigma((g_1, g_2, \dots, g_{p - 1}, g_0)) = (g_0, g_1, \dots, g_{p - 1}) = g \\\\
    (\upsilon \circ \sigma)(g) = \upsilon(\sigma(g)) = \upsilon(g_{p - 1}, g_0, g_1, \dots, g_{p - 2})) = (g_0, g_1, \dots, g_{p - 1}) = g \\\\
    \implies \upsilon = \sigma^{-1} \implies \sigma \text { е биекция от } M \text{ в } M \)
    \subsection*{в)}
    \(H = \cycleG{\sigma} < S_M \implies |H| = |\sigma| \\\\
    g \in M \implies g = (g_0, g_1, \dots, g_{p - 1}), \; g_i \in G, \; i = 0, \dots, {p - 1} \\\\
    \sigma(g) = \sigma((g_0, g_1, \dots, g_{p - 1})) = (g_{p - 1}, g_0, g_1, \dots, g_{p - 2}) \\\\
    (\sigma^2)(g) = \sigma(\sigma(g))) = \sigma((g_{p - 1}, g_0, g_1, \dots, g_{p - 2})) = (g_{p - 2}, g_{p - 1}, g_0, g_1, \dots, g_{p - 3}) \\\\
    (\sigma^3)(g) = \sigma(\sigma(\sigma(g)))) = \sigma((g_{p - 2}, g_{p - 1}, g_0, g_1, \dots, g_{p - 3})) = (g_{p - 3}, g_{p - 2}, g_{p - 1}, g_0, g_1, \dots, g_{p - 4}) \\\\
    \implies (\sigma^i)(g) = \sigma^i((g_0, g_1, \dots, g_{p - 1})) = (g_{(-i \; mod \; p)}, g_{(1 - i \; mod \; p)}, \dots, g_{(p - 1 - i \; mod \; p)}) \implies \\\\
    \sigma^i = id \iff -i \equiv 0 \; \pmod{p} \implies i = p = min\{q \in \N \; | \; \sigma^q = id \} \implies \\\\
    (\sigma^p)(g) = id(g) \implies |\sigma| = p \implies |H| = p\)
    \subsection*{г)}
    \(\begin{array}{cccc}
    \varphi : & H \times M  & \to & M \\
     ~ &  (\rho, m) & \mapsto & \rho(m)
    \end{array} \\\\
    \forall g \in M \quad \varphi(id, g) = id(g) = g \\\\
    \forall g \in M, \; \forall \sigma^i, \sigma^j, \;  i, j \in \Z \quad \varphi(\sigma^i, \varphi(\sigma^j, g)) = \\\\
    = \varphi(\sigma^i, \sigma^j(g)) = \sigma^i(\sigma^j(g)) = (\sigma^i\sigma^j)(g) = \varphi(\sigma^i\sigma^j, g)\)
    \subsection*{д)}
    \(St((g_0, g_1, \dots, g_{p- 1})) = \{h \in H \; | \; \varphi(h, (g_0, g_1, \dots, g_{p- 1})) = (g_0, g_1, \dots, g_{p - 1})\} \\\\
    St((g_0, g_1, \dots, g_{p - 1})) = H \iff \forall \sigma^i \neq id \in H, \; i \in \Z, \; 0 < i < p \\\\
    \sigma^i((g_0, g_1, \dots, g_{p - 1})) = (g_{(-i \; mod \; p)}, g_{(1 - i \; mod \; p)}, \dots, g_{(p - 1 - i \; mod \; p)}) = \\\\
    = (g_0, g_1, \dots, g_{p - 1}) \iff \left\vert\begin{array}{l}
    	g_0 = g_1 = \dots = g_{p - 1} = g_s \\
    	~ \\
    	g_s^p = e_G
    \end{array}\right. \iff g_s = e_G \vee |g_s| = p  \)
    \subsection*{е)}
    \(\forall g \in M \; O(g) = \{\varphi(h, g) \; | \; h \in H\} \implies O(x) = O(y) \iff x \sim y \\\\
    \forall a, b \in M \; \; a = (a_0, a_1, \dots a_{p - 1}), \; b = (b_0, b_1, \dots b_{p - 1}) \implies \\\\
    a \sim b \iff \{a_0, a_1, \dots a_{p - 1}\} = \{b_0, b_1, \dots b_{p - 1}\} \\\\
    St(g) = \{h \in H \; | \; \varphi(h, g) = g)\} \\\\
    h_1, h_2 \in H \varphi(h_1, g) = \varphi(h_2, g) \iff h_1(g) = h_2(g) \iff \\\\
    (h_2^{-1}h_1)(g) = g \iff h_2^{-1}h_1 \in St(g) \iff h_1St(g) = h_2St(g) \implies \\\\
    |O(g)| = |H : St(g)| \implies |O(g)| | |H| \\\\
    |H| = p \implies |O(g)| = 1 \vee |O(g)| = p \implies \\\\
    |M| = n^{p - 1} = s.1 + o.p, \; s, o \in \N, \; s \geq 1 (\;(e_G, e_G, \dots, e_G) \in M)\;) \\\\
    p|n \implies p|s \implies \\\\
    \exists S = \{v = (x, x, \dots, x) \in M \; | \; |O(v)| = 1, \; x^p = e_G\}; \; |S| \geq p \implies \\\\
    \exists Y = \{y \in G \; | \; y^p = e_G\}; \; |Y| \geq p \implies \\\\  
    \exists u \in G;  \; u \neq e_G, \; u^p = e_G \implies \; |u| = p\)
\end{document}
