\documentclass{article}
\usepackage{amsmath}
\usepackage{amssymb}
\usepackage[T1,T2A]{fontenc}
\usepackage[utf8]{inputenc}
\usepackage[bulgarian]{babel}
\usepackage[normalem]{ulem}
\usepackage{tikz}

\newcommand{\vectr}{\overrightarrow}
\newcommand{\stkout}[1]{\ifmmode\text{\sout{\ensuremath{#1}}}\else\sout{#1}\fi}

\begin{document}
    \pagenumbering{gobble}
    \begin{tikzpicture}
    \draw (5,1) node[anchor=west]{$A(5, 1)$}
        -- (3,3) node[anchor=west]{$B(3, 3)$}
        -- (-1,5) node[anchor=west]{$C(-1, 5)$}
        -- cycle;
    \draw (7/2, 3/2) node[anchor=north]{$S_{AB}$} -- (4, 2) node[anchor=west]{$M(4, 2)$};
    \draw (8/3, 4) node[anchor=east]{$S_{AC}$} -- (2, 3) node[anchor=east]{$N(2, 3)$};
    \end{tikzpicture}
    \\\(A(5, 1), \; B(3, 3) \; C(-1, 5)\\
    \\S_{AB}, \; S_{AC} = ?\\
    \\S_{AB} \cap S_{AC} = ?\\
    \\R = ?\\
    \\S_{AB} : \begin{cases}
        z \; M\\
        \perp AB
    \end{cases}\\
    \\M(\frac{5 + 3}{2}, \frac{1 + 3}{2}) \implies M(4, 2)\\
    \\AB : \begin{cases}
        z \; A(5, 1)\\
        z \; B(3, 3)
    \end{cases}
    \\AB : \begin{vmatrix}
        x - 3 & y - 3\\
        2 &  -2
    \end{vmatrix} = 0\\
    \\AB : -2x + 6 -2y + 6 = 0\\
    \\AB: -2x -2y + 12 = 0 \; |-\frac{1}{2}\\
    \\AB : x + y + 6 = 0\\
    \\S_{AB} \perp AB \implies S_{AB} : -x + y + C = 0\\
    \\M(4, 2) \; z \; S_{AB} \implies -4 + 2 + C = 0\\
    \\\implies S_{AB} : -x + y + 2 = 0\\
    \\S_{AC} : \begin{cases}
        z \; N\\
        \perp AC
    \end{cases}\\
    \\N(\frac{5 - 1}{2}, \frac{1 + 5}{2}) \implies N(2, 3)\\
    \\AC : \begin{cases}
        z \; A(5, 1)\\
        z \; C(-1, 5)
    \end{cases}
    \\AB : \begin{vmatrix}
        x - 5 & y - 1\\
        -6 &  4
    \end{vmatrix} = 0\\
    \\AC : 4x - 20 + 6y - 6 = 0\\
    \\AC : 4x + 6y - 26 = 0 \; |\frac{1}{2}\\
    \\AC : 2x + 3y - 13 = 0\\
    \\S_{AC} \perp AC \implies S_{AC} : -3x + 2y + C = 0\\
    \\N(2, 3) \; z \; S_{AC} \implies -6 + 6 + C = 0\\
    \\\implies S_{AC} : -3x + 2y = 0\\
    \\S_{AB} \cap S_{AC} = O(x_O, y_O)\\
    \\\begin{array}{lcl}
        -3x_O + 2y_O & = & 0\\
        -x_O + y_O + 2 & = & 0 \; |-3
    \end{array}\\
    \\\\\begin{array}{lcl}
        -3x_s + 2y_O & = & 0\\
        3x_O - 3y_O - 6 & = & 0
    \end{array}\\
    \\ y_O = -6 \implies x_O = -4 \implies O(-4, -6)\\
    \\\vectr{BS}(-7, -9)\\
    \\|\vectr{BS}| = \sqrt{49 + 81} = \sqrt{130} = R\)
\end{document}
